Patched holes in ParserADT.

src/Parsers/ParserADT.v
@@ -1,16 +1,17 @@
-(** * Reference implementation of a splitter and parser based on that splitter *)
+(* Reference implementation of a splitter and parser based on that splitter *)
 Require Import ADTNotation.BuildADT ADTNotation.BuildADTSig.
 Require Import ADT.ComputationalADT.
 Require Import ADTSynthesis.Common.List.Operations.
 Require Import ADTRefinement.GeneralRefinements.
 Require Import Parsers.ParserInterface.
+Require Import ADTSynthesis.ADTRefinement.Core.
 
 Set Implicit Arguments.
 
 Local Open Scope list_scope.
 Local Open Scope ADTSig_scope.
 Local Open Scope ADT_scope.
-
+Local Open Scope string_scope.
 Section ReferenceImpl.
   Context {CharType} {String : string_like CharType} (G : grammar CharType).
 
@@ -46,22 +47,56 @@ Section ReferenceImpl.
   }.
 
   Section parser.
-    Context (splitter : Sharpened string_spec).
 
-    Local Obligation Tactic := admit.
+    Context (splitter_impl : cADT string_rep)
+            (splitter_OK   : refineADT string_spec (LiftcADT splitter_impl)).
+    Local Obligation Tactic := idtac.
+    (* Don't want it inferring silly method implementations. *)
 
     Program Definition adt_based_splitter : Splitter String G
-      := {| split_rep := _ (* rep of splitter *);
+      := {| split_rep := cRep splitter_impl (* rep of splitter *);
             split_take n st := _ (* call "take"(st, n) on splitter *);
             split_drop n st := _ (* call "drop"(st, n) on splitter *);
             splits_for st it its := _ (* call "splits"(st, (it, its)) on splitter *);
-            split_invariant str st := _ (* rep inv between String and split_rep *);
+            split_invariant str st := AbsR (splitter_OK) str st (* rep inv between String and split_rep *);
             take_respectful str st n H := _ (* proof that "take" preserves the rep inv w.r.t. its spec *);
             drop_respectful str st n H := _ (* proof that "drop" preserves the rep inv w.r.t. its spec *);
             splits_for_complete str st it its H := _ (* proof that "splits" obeys its spec, given that the rep inv holds on the input, by H *) |}.
-    (* Next Obligation.
-    Proof.
-    ...
-    Qed. *)
+    Next Obligation.
+      let impl := eval simpl in
+      (fun n st => fst (cMethods splitter_impl {| StringBound.bindex := "take" |} st n)) in
+          exact impl.
+    Defined.
+    Next Obligation.
+      let impl := eval simpl in
+      (fun n st => fst (cMethods splitter_impl {| StringBound.bindex := "drop" |} st n)) in
+          exact impl.
+    Defined.
+    Next Obligation.
+      let impl := eval simpl in
+      (fun st it its => snd (cMethods splitter_impl {| StringBound.bindex := "splits" |} st (it, its))) in
+          exact impl.
+    Defined.
+    Next Obligation.
+      intros.
+      pose proof (ADTRefinementPreservesMethods splitter_OK {|StringBound.bindex := "take" |} _ _ n H ((cMethods splitter_impl {| StringBound.bindex := "take" |} st n)) (ReturnComputes _)).
+      computes_to_inv; injections; simpl in *; subst.
+      computes_to_inv; subst; simpl in *.
+      unfold adt_based_splitter_obligation_1; rewrite <- H0''; eauto.
+    Qed.
+    Next Obligation.
+      intros.
+      pose proof (ADTRefinementPreservesMethods splitter_OK {|StringBound.bindex := "drop" |} _ _ n H ((cMethods splitter_impl {| StringBound.bindex := "drop" |} st n)) (ReturnComputes _)).
+      computes_to_inv; injections; simpl in *; subst.
+      computes_to_inv; subst; simpl in *.
+      unfold adt_based_splitter_obligation_2; rewrite <- H0''; eauto.
+    Qed.
+    Next Obligation.
+      intros.
+      pose proof (ADTRefinementPreservesMethods splitter_OK {|StringBound.bindex := "splits" |} _ _ (it, its) H ((cMethods splitter_impl {| StringBound.bindex := "splits" |} st (it, its))) (ReturnComputes _)).
+      computes_to_inv; injections; simpl in *; subst.
+      computes_to_inv; subst; simpl in *.
+      unfold adt_based_splitter_obligation_3; rewrite <- H0''; eauto.
+    Qed.
   End parser.
 End ReferenceImpl.
